

## Exercise 1

$$\begin{aligned}P(B) &= 0.01 \\P(\neg B) &= 1 - P(B) = 1 - 0.01 = 0.99\end{aligned}$$

$$\begin{aligned}P(\text{Test} = \text{positive}|B) &= 0.95 \\P(\text{Test} = \text{negative}|B) &= 1 - P(\text{Test} = \text{positive}|B) = 0.05 \\P(\text{Test} = \text{positive}|\neg B) &= 1 - P(\text{Test} = \text{negative}|\neg B) = 0.1 \\P(\text{Test} = \text{negative}|\neg B) &= 0.9\end{aligned}$$

## Solution A

$$\begin{aligned}P(B|\text{Test} = \text{positive}) &\stackrel{\text{Bayes}}{=} \frac{P(\text{Test} = \text{positive}|B) * P(B)}{P(\text{Test} = \text{positive})} \\&\stackrel{\text{T.P.F}}{=} \frac{P(\text{Test} = \text{positive}|B)P(B)}{P(\text{Test} = \text{positive})P(B) + P(\text{Test} = \text{positive}|\neg B)P(\neg B)} \\&= \frac{0.95 * 0.01}{0.95 * 0.01 + 0.10 * 0.99} \\&= \frac{0.0095}{0.0095 + 0.0990} \\&\approx 0.0876\end{aligned}$$

## Solution B

$$P(B|\text{Test} = \text{positive}) = 0.5$$

$$\begin{aligned}
P(B|Test = positive) &\stackrel{Bayes}{=} \frac{P(Test = positive|B) * P(B)}{P(Test = positive)} \\
&\stackrel{T.P.F}{=} \frac{P(Test = positive|B)P(B)}{P(Test = positive)P(B) + P(Test = positive|\neg B)P(\neg B)} \\
&= \frac{[P(Test = positive)P(B) + P(Test = positive|\neg B)P(\neg B)]}{P(B|Test = positive) = P(Test = positive|B)P(B)} \\
&= \frac{P(Test = positive)P(B) + P(Test = positive|\neg B)P(\neg B)}{P(B|Test = positive)} \\
&= \frac{P(Test = positive|B)P(B)}{P(B|Test = positive)} - P(Test = positive)P(B) \\
&= \frac{P(Test = positive|B)P(B)}{P(\neg B)} \left( \frac{1}{P(B|Test = positive)} - 1 \right) \\
&= \frac{P(Test = positive|B)P(B)}{P(\neg B)} \left( \frac{1}{P(B|Test = positive)} - 1 \right) \\
&= 1 - \frac{P(Test = positive|B)P(B)}{P(\neg B)} \left( \frac{1}{P(B|Test = positive)} - 1 \right) \\
&= 1 - \frac{0.95 * 0.01}{0.99} \left( \frac{1}{0.5} - 1 \right) \\
&= 1 - \frac{0.95 * 0.01}{0.99} \\
&= 1 - \frac{0.0095}{0.99} \\
&\approx 1 - 0.0095 \\
&= 0.9905
\end{aligned}$$